pulse/src/checker/Pulse.Syntax.Pure.fst
@@ -472,3 +472,24 @@ let rec list_as_vprop (vps:list term)
     | [] -> tm_emp
     | [hd] -> hd
     | hd::tl -> tm_star hd (list_as_vprop tl)
+
+let rec insert1 (t:term) (ts : list term) : T.Tac (list term) =
+  match ts with
+  | [] -> [t]
+  | t'::ts' ->
+    if Order.le (T.compare_term t t')
+    then t::ts
+    else t'::insert1 t ts'
+
+let sort_terms (ts : list term) : T.Tac (list term) =
+  T.fold_right insert1 ts []
+
+(* This does not have any useful lemmas, but can put the terms
+in order. It's useful to pretty-print contexts. See #96. *)
+let canon_vprop_list_print (vs : list term)
+  : T.Tac term
+  = list_as_vprop <| sort_terms vs
+
+let canon_vprop_print (vp:term)
+  : T.Tac term
+  = canon_vprop_list_print <| vprop_as_list vp
